LeanMqtt/Primitives/OptType/Basic.lean
@@ -1,0 +1,37 @@
+import LeanMqtt.Core.Codec
+
+namespace Mqtt
+open Mqtt
+
+/--
+  `OptType` is a generic primitive for conditionally present fields.
+  It evaluates definitionally to `α` when `b` is `true`, and `Unit` when `b` is `false`.
+
+  At first glance, using `Bool` instead of  `Prop` might seem like it may wield incorrect
+  results. What prevents a buggy parser from evaluating always passing `false` and breaking
+  the protocol?
+
+  The guarantee is preserved because the boolean is embedded directly into the type
+  signature of the parent structure.
+
+  For example, if we declare the following, from `VarHeader/Variations.lean`:
+  ```
+  packet_id : OptType UInt16 (qos.val > 0)
+  ```
+
+  Any parser or serializer that passes a different condition will yield a mismatched type
+  (e.g., `OptType UInt16 false`). Lean's typechecker will catch this mismatch and reject
+  the implementation.
+-/
+abbrev OptType (α : Type) (b : Bool) : Type :=
+  cond b α Unit
+
+def OptType.serialize {α : Type} [c : Codec α] (b : Bool) (v : OptType α b) : List UInt8 :=
+  match b, v with
+  | true,  val => @Codec.serialize α c val
+  | false, _   => []
+
+def OptType.parser {α : Type} [c : Codec α] (b : Bool) : Parser (OptType α b) :=
+  match b with
+  | true  => @Codec.parser α c
+  | false => pure ()
