LeanMqtt/Primitives/OptType/Proofs.lean
@@ -1,0 +1,24 @@
+import LeanMqtt.Core.Codec
+import LeanMqtt.Primitives.OptType.Basic
+
+namespace Mqtt
+open Mqtt
+
+theorem OptType.roundtrip {α : Type} [c : Codec α] (b : Bool) (v : OptType α b) {rest : List UInt8} :
+    (OptType.parser b).run (serialize b v ++ rest) = some (v, rest) := by
+  match b, v with
+  | true,  val =>
+    exact @Codec.roundtrip α c val rest
+  | false, ()  =>
+    rfl
+
+theorem OptType.reconstruct {α : Type} [c : Codec α]
+    (b : Bool) {v : OptType α b} {input rest : List UInt8} :
+    (OptType.parser b).run input = some (v, rest) → input = serialize b v ++ rest := by
+  intro h
+  match b, v, h with
+  | true, val, h =>
+    exact @Codec.reconstruct α c val input rest h
+  | false, (), h =>
+    injection h with h_pair
+    injection h_pair with _ _
